\documentclass[11pt,letterpaper]{article}
\usepackage[left=1.00in, right=1.00in, top=1.00in, bottom=1.00in]{geometry}

\usepackage{mathrsfs}
\usepackage{mathtools}

\usepackage{amsmath}
\usepackage{amsfonts}
\usepackage{amssymb}

\begin{document}

\noindent
Math W80 Homework \hfill Micah Ng \hfill \today

\begin{center}
\line(1, 0){250}
\end{center}

\noindent
Homework 1

\begin{enumerate}
\item
  \begin{enumerate}
  \item
    \begin{align*}
      \mathbf{v} &= c_1\mathbf{u}_1+c_2\mathbf{u}_2+\cdots+c_n\mathbf{u}_n \\
      \langle\mathbf{v}, \mathbf{u}_j\rangle &= \langle c_1\mathbf{u}_1+\cdots+c_n\mathbf{u}_n, \mathbf{u}_j\rangle \\
          &= \langle c_1\mathbf{u}_1, \mathbf{u}_j\rangle+\cdots+\langle c_n\mathbf{u}_n, \mathbf{u}_j\rangle \\
          &= c_1\langle\mathbf{u}_1, \mathbf{u}_j\rangle+\cdots+c_n\langle\mathbf{u}_n, \mathbf{u}_j\rangle \\
          &= c_j\langle\mathbf{u}_j, \mathbf{u}_j\rangle \tag{since $\mathbf{u}$ is pairwise orthogonal} \\
      c_j &= \frac{\langle\mathbf{v}, \mathbf{u}_j\rangle}{|\mathbf{u}_j|^2}
    \end{align*}

  \item
    \begin{align*}
      \mathbf{0} &= c_1\mathbf{u}_1+\cdots+c_n\mathbf{u}_n \\
      c_j &= \frac{\langle\mathbf{0}, \mathbf{u}_j\rangle}{|\mathbf{u}_j|^2} \\
          &= 0
    \end{align*}
    Thus all coefficients must be 0, showing that
    $\mathbf{u}_1,\ldots,\mathbf{u}_n$ are linearly independent.

  \item
    $\mathbf{U}^{-1}$ is the matrix with rows, in order,
    $\frac{\mathbf{u}_1}{|\mathbf{u}_1|^2},\ldots,\frac{\mathbf{u}_n}{|\mathbf{u}_n|^2}$.
    So, each cell of $\mathbf{U}^{-1}\mathbf{U}$ is
    \begin{align*}
      \left\langle\frac{\mathbf{u}_i}{|\mathbf{u}_i|^2},\mathbf{u}_j\right\rangle
          &= \frac{\left\langle\mathbf{u}_i,\mathbf{u}_j\right\rangle}{|\mathbf{u}_i|^2}
    \end{align*}
    If $i=j$, then the cell is along the diagonal, and
    $\frac{\left\langle\mathbf{u}_i,\mathbf{u}_i\right\rangle}{|\mathbf{u}_i|^2}=\frac{|\mathbf{u}_i|^2}{|\mathbf{u}_i|^2}=1$.
    If $i\neq j$, then the cell is not on the diagonal, and
    $\frac{\left\langle\mathbf{u}_i,\mathbf{u}_j\right\rangle}{|\mathbf{u}_i|^2}=\frac{0}{|\mathbf{u}_i|^2}=0$.

    This verifies that $\mathbf{U}^{-1}\mathbf{U}=\mathbf{I}$ holds.
  \end{enumerate}

\item
  \begin{enumerate}
  \item
    
  \end{enumerate}
\end{enumerate}

\begin{center}
\line(1, 0){250}
\end{center}


\end{document}
